Roughly fix flatten_correct

compiler/backend/proofs/stack_to_labProofScript.sml
@@ -108,8 +108,7 @@ val state_rel_def = Define`
     (!k n. k ∈ s.ffi_save_regs ==> t.cc_regs n k = NONE) /\
     (∀x. x ∈ s.mdomain ⇒ w2n x MOD (dimindex (:'a) DIV 8) = 0) ∧
     s.code_buffer = t.code_buffer ∧
-    (* TODO: this ordinarily would set c to a pair, which seems inconvenient *)
-    s.compile = (λc (p,_). t.compile c (MAP prog_to_section p)) ∧
+    s.compile = (λc p. t.compile c (MAP prog_to_section p)) ∧
     (t.compile_oracle = λn. let (c,p,_)  = s.compile_oracle n in
                            (c,MAP prog_to_section p)) ∧
     (∀k. let (c,p,_) = s.compile_oracle k in
@@ -364,6 +363,70 @@ val halt_view_def = Define`
   (halt_view _ = NONE)`;
 val _ = export_rewrites["halt_view_def"];
 
+(* TODO: these are probably already proved in lab_filter or lab_to_target,
+         they ought to move into labProps
+*)
+val asm_fetch_aux_SOME_append = Q.prove(`
+  ∀pc code l code2.
+  asm_fetch_aux pc code = SOME l ⇒
+  asm_fetch_aux pc (code++code2) = SOME l`,
+  ho_match_mp_tac asm_fetch_aux_ind>>simp[asm_fetch_aux_def]>>rw[]);
+
+val asm_fetch_aux_SOME_isPREFIX = Q.prove(`
+  ∀pc code l code2.
+  asm_fetch_aux pc code = SOME l /\
+  code ≼ code2 ==>
+  asm_fetch_aux pc code2 = SOME l`,
+  rw[]>>fs[IS_PREFIX_APPEND]>>
+  metis_tac[asm_fetch_aux_SOME_append]);
+
+val loc_to_pc_APPEND = Q.store_thm("loc_to_pc_APPEND",`
+  ∀n m code pc code2.
+  loc_to_pc n m code = SOME pc ⇒
+  loc_to_pc n m (code ++ code2) = SOME pc`,
+  ho_match_mp_tac loc_to_pc_ind>>rw[]
+  >-
+    fs[loc_to_pc_def]
+  >>
+  simp[Once loc_to_pc_def]>>
+  rw[]
+  >-
+    fs[Once loc_to_pc_def]
+  >>
+  TOP_CASE_TAC>>fs[]>>rfs[]>>
+  TRY(fs[Once loc_to_pc_def]>>rfs[]>>NO_TAC)>>
+  rw[]>>rfs[]>>qpat_x_assum`_=SOME pc` mp_tac>>
+  simp[Once loc_to_pc_def]>>fs[]>>
+  TOP_CASE_TAC>>rw[]>>
+  fs[]);
+
+val code_installed_APPEND = Q.store_thm("code_installed_APPEND",`
+  ∀ls pc code code2.
+  code_installed pc ls code ==>
+  code_installed pc ls (code ++ code2)`,
+  Induct>>simp[code_installed_def]>> rw[]
+  >-
+    (TOP_CASE_TAC>>fs[is_Label_def]>>
+    metis_tac[loc_to_pc_APPEND])
+  >>
+    metis_tac[asm_fetch_aux_SOME_append]);
+
+val code_installed_isPREFIX = Q.store_thm("code_installed_isPREFIX",`
+  ∀ls pc code code2.
+  code_installed pc ls code ∧
+  code ≼ code2 ==>
+  code_installed pc ls code2`,
+  rw[]>>
+  fs[IS_PREFIX_APPEND]>>
+  metis_tac[code_installed_APPEND]);
+
+val loc_to_pc_isPREFIX = Q.store_thm("loc_to_pc_isPREFIX",`
+  ∀n m code pc code2.
+  loc_to_pc n m code = SOME pc /\
+  code ≼ code2 ==>
+  loc_to_pc n m code2 = SOME pc`,
+  rw[]>>fs[IS_PREFIX_APPEND]>>metis_tac[loc_to_pc_APPEND]);
+
 val finish_tac =
   rename1`halt_view (SOME z)` \\ Cases_on`z` \\ fs[] >>
   imp_res_tac loc_to_pc_isPREFIX>>
@@ -402,70 +465,6 @@ val finish_tac =
   first_x_assum(qspec_then`ck'`mp_tac) \\ simp[];
 
 val call_args_def = stackPropsTheory.call_args_def;
-
-(* TODO: these are probably already proved in lab_filter or lab_to_target,
-         they ought to move into labProps
-*)
-val asm_fetch_aux_SOME_append = Q.prove(`
-  ∀pc code l code2.
-  asm_fetch_aux pc code = SOME l ⇒
-  asm_fetch_aux pc (code++code2) = SOME l`,
-  ho_match_mp_tac asm_fetch_aux_ind>>simp[asm_fetch_aux_def]>>rw[]);
-
-val asm_fetch_aux_SOME_isPREFIX = Q.prove(`
-  ∀pc code l code2.
-  asm_fetch_aux pc code = SOME l /\
-  code ≼ code2 ==>
-  asm_fetch_aux pc code2 = SOME l`,
-  rw[]>>fs[IS_PREFIX_APPEND]>>
-  metis_tac[asm_fetch_aux_SOME_append]);
-
-val loc_to_pc_APPEND = Q.store_thm("loc_to_pc_APPEND",`
-  ∀n m code pc code2.
-  loc_to_pc n m code = SOME pc ⇒
-  loc_to_pc n m (code ++ code2) = SOME pc`,
-  ho_match_mp_tac loc_to_pc_ind>>rw[]
-  >-
-    fs[loc_to_pc_def]
-  >>
-  simp[Once loc_to_pc_def]>>
-  rw[]
-  >-
-    fs[Once loc_to_pc_def]
-  >>
-  TOP_CASE_TAC>>fs[]>>rfs[]>>
-  TRY(fs[Once loc_to_pc_def]>>rfs[]>>NO_TAC)>>
-  rw[]>>rfs[]>>qpat_x_assum`_=SOME pc` mp_tac>>
-  simp[Once loc_to_pc_def]>>fs[]>>
-  TOP_CASE_TAC>>rw[]>>
-  fs[]);
-
-val loc_to_pc_isPREFIX = Q.store_thm("loc_to_pc_isPREFIX",`
-  ∀n m code pc code2.
-  loc_to_pc n m code = SOME pc /\
-  code ≼ code2 ==>
-  loc_to_pc n m code2 = SOME pc`,
-  rw[]>>fs[IS_PREFIX_APPEND]>>metis_tac[loc_to_pc_APPEND]);
-
-val code_installed_APPEND = Q.store_thm("code_installed_APPEND",`
-  ∀ls pc code code2.
-  code_installed pc ls code ==>
-  code_installed pc ls (code ++ code2)`,
-  Induct>>simp[code_installed_def]>> rw[]
-  >-
-    (TOP_CASE_TAC>>fs[is_Label_def]>>
-    metis_tac[loc_to_pc_APPEND])
-  >>
-    metis_tac[asm_fetch_aux_SOME_append]);
-
-val code_installed_isPREFIX = Q.store_thm("code_installed_isPREFIX",`
-  ∀ls pc code code2.
-  code_installed pc ls code ∧
-  code ≼ code2 ==>
-  code_installed pc ls code2`,
-  rw[]>>
-  fs[IS_PREFIX_APPEND]>>
-  metis_tac[code_installed_APPEND]);
 
 val MAP_prog_to_section_FST = Q.prove(`
   MAP (λs. case s of Section n v => n) (MAP prog_to_section prog) =
@@ -1488,21 +1487,15 @@ val flatten_correct = Q.store_thm("flatten_correct",
       simp[upd_pc_def,dec_clock_def,Abbr`ss`] >>
       first_x_assum(qspec_then`ck1`mp_tac)>>simp[] >>
       NO_TAC)) >>
-  (* InstallAndRun *)
+  (* Install *)
   conj_tac >- (
     rw[stackSemTheory.evaluate_def]>>
     fs[case_eq_thms]>>
     pairarg_tac>>fs[]>>
     fs[get_var_def]>>
     imp_res_tac state_rel_read_reg_FLOOKUP_regs>>
-    fs[case_eq_thms]
-    >-
-      (* Timeout *)
-      (qexists_tac`0`>>
-      qexists_tac`t1`>>
-      fs[state_rel_def])>>
-    rw[]>>
-    rfs[]>>
+    fs[case_eq_thms]>>
+    rw[]>> rfs[]>>
     qpat_x_assum`code_installed _ _ _` mp_tac>>
     simp[Once flatten_def]>> strip_tac>>
     fs[code_installed_def]>>
@@ -1510,119 +1503,91 @@ val flatten_correct = Q.store_thm("flatten_correct",
     simp[Once state_rel_def]>>
     strip_tac>>fs[prog_to_section_def]>>
     pairarg_tac>>fs[]>>
-    `t1.clock ≠ 0` by fs[state_rel_def]>>
     qmatch_asmsub_abbrev_tac`t1.compile cfg new_code`>>
     (* Have to assume that none of the new sections have appeared before *)
     `?pc. loc_to_pc k 0
               (t1.code ++ new_code) = SOME pc ∧
           code_installed pc (append lines) (t1.code ++ new_code)` by
       cheat>>
+    rw[]>>qexists_tac`2`>>
+    simp[Once labSemTheory.evaluate_def]>>
+    simp[asm_fetch_def]>>
+    fs[call_args_def]>>rw[]>>fs[]>>simp[]>>
+    fs[get_pc_value_def,lab_to_loc_def]>>
+    simp[inc_pc_def,dec_clock_def,upd_reg_def]>>
+    (* Do the install *)
+    simp[Once labSemTheory.evaluate_def]>>
+    simp[asm_fetch_def]>>
+    simp[APPLY_UPDATE_THM]>>
+    qpat_x_assum`Word _ = _` (assume_tac o SYM)>>
+    qpat_x_assum`Word _ = _` (assume_tac o SYM)>>
+    fs[prog_to_section_def,shift_seq_def]>>
+    pairarg_tac>>fs[]>>
     qabbrev_tac `tt = t1 with
         <|regs :=
             (t1.ptr_reg =+ Loc k 0)
               (λa.
                  get_reg_value (t1.cc_regs 0 a)
                    (if t1.link_reg = a then Loc n l
-                    else read_reg a t1) Word); pc := pc;
+                    else read_reg a t1) Word); pc := t1.pc+2;
           cc_regs := shift_seq 1 t1.cc_regs;
           code :=
             t1.code ++
             Section k (append lines ++ [Label k m 0])::
-                MAP prog_to_section v8;
+                MAP prog_to_section v7;
           compile_oracle := shift_seq 1 t1.compile_oracle;
           code_buffer := cb;
-          clock:=t1.clock-1|>`>>
-    first_x_assum(qspecl_then [`k`,`next_lab prog 1`,`tt`] mp_tac)>>
-    impl_tac>-
-      (fs[shift_seq_def]>>
-      simp[state_rel_def,Abbr`tt`,stackSemTheory.dec_clock_def]>>
-      rw[]
-      >-
-        (fs[APPLY_UPDATE_THM,FLOOKUP_DRESTRICT,FLOOKUP_UPDATE,call_args_def]>>
-        pop_assum mp_tac>>
-        IF_CASES_TAC>-
-          simp[]>>
-        IF_CASES_TAC>-
-          (simp[get_reg_value_def]>>
-          rw[]>>fs[])>>
-        simp[])
-      >-
-        (fs[lookup_union,case_eq_thms]
-        >-
-          (qmatch_asmsub_abbrev_tac`fromAList pp`>>
-          fs[lookup_fromAList]>>
-          imp_res_tac ALOOKUP_MEM>>
-          first_x_assum(qspec_then`0` assume_tac)>>
-          rfs[EVERY_MEM,FORALL_PROD]>>
-          metis_tac[])
-        >>
-          metis_tac[])
-      >-
-        (pop_assum mp_tac>>simp[lookup_union]>>
-        reverse TOP_CASE_TAC>> strip_tac
-        >-
-          (first_x_assum drule>>rw[]>>
-          metis_tac[loc_to_pc_APPEND,code_installed_APPEND])
-        >>
-          cheat)
-      >-
-        (pairarg_tac>>fs[]>>
-        first_x_assum(qspec_then`k'+1` assume_tac)>>rfs[]>>
-        fs[GSYM ADD1,GENLIST_CONS]>>
-        rfs[Abbr`new_code`,MAP_prog_to_section_Section_num]>>
-        fs[o_DEF])
-      >-
-        (first_x_assum(qspec_then`0` assume_tac)>>
-        rfs[EVERY_MEM,FORALL_PROD]))>>
-    rw[]>>qexists_tac`ck+2`>>
-    reverse TOP_CASE_TAC>>fs[]
+          clock:=t1.clock|>`>>
+    qexists_tac`tt` >>
+    fs[Abbr`tt`]>>
+    CONJ_TAC>-
+      (rw[]>>fs[shift_seq_def,Abbr`new_code`])>>
+    CONJ_TAC>-
+      simp[append_def,append_aux_def,flatten_def]>>
+    fs[state_rel_def]>>
+    rw[]
     >-
-      (* Do the jump *)
-      (simp[Once labSemTheory.evaluate_def]>>
-      simp[asm_fetch_def]>>
-      fs[call_args_def]>>rw[]>>fs[]>>simp[]>>
-      fs[get_pc_value_def,lab_to_loc_def]>>
-      simp[inc_pc_def,dec_clock_def,upd_reg_def]>>
-      (* Do the install *)
-      simp[Once labSemTheory.evaluate_def]>>
-      simp[asm_fetch_def]>>
-      simp[APPLY_UPDATE_THM]>>
-      qpat_x_assum`Word _ = _` (assume_tac o SYM)>>
-      qpat_x_assum`Word _ = _` (assume_tac o SYM)>>
-      fs[prog_to_section_def,shift_seq_def]>>
-      pairarg_tac>>fs[]>>
-      (* Do the actual call *)
-      simp[Once labSemTheory.evaluate_def]>>
-      imp_res_tac asm_fetch_aux_SOME_append>>
-      simp[asm_fetch_def,APPLY_UPDATE_THM]>>
-      simp[upd_pc_def,dec_clock_def]>>
-      rfs[Abbr`tt`])
-    >>
-      simp[Once labSemTheory.evaluate_def]>>
-      simp[asm_fetch_def]>>
-      fs[call_args_def]>>rw[]>>fs[]>>simp[]>>
-      fs[get_pc_value_def,lab_to_loc_def]>>
-      simp[inc_pc_def,dec_clock_def,upd_reg_def]>>
-      (* Do the install *)
-      simp[Once labSemTheory.evaluate_def]>>
-      simp[asm_fetch_def]>>
-      simp[APPLY_UPDATE_THM]>>
-      qpat_x_assum`Word _ = _` (assume_tac o SYM)>>
-      qpat_x_assum`Word _ = _` (assume_tac o SYM)>>
-      fs[prog_to_section_def,shift_seq_def]>>
-      pairarg_tac>>fs[]>>
-      (* Do the actual call *)
-      simp[Once labSemTheory.evaluate_def]>>
-      imp_res_tac asm_fetch_aux_SOME_append>>
-      simp[asm_fetch_def,APPLY_UPDATE_THM]>>
-      simp[upd_pc_def,dec_clock_def]>>
-      rfs[Abbr`tt`]>>
-      rfs[]>>
-      qexists_tac`t2`>>
-      CONJ_TAC>-
+      (fs[APPLY_UPDATE_THM,FLOOKUP_DRESTRICT,FLOOKUP_UPDATE,call_args_def]>>
+      pop_assum mp_tac>>
+      IF_CASES_TAC>-
         simp[]>>
-      simp[]>>
-      metis_tac[IS_PREFIX_TRANS,IS_PREFIX_APPEND])>>
+      IF_CASES_TAC>-
+        (simp[get_reg_value_def]>>
+        rw[]>>fs[])>>
+      simp[])
+    >-
+      (fs[lookup_union,case_eq_thms]
+      >-
+        (qmatch_asmsub_abbrev_tac`fromAList pp`>>
+        fs[lookup_fromAList]>>
+        imp_res_tac ALOOKUP_MEM>>
+        first_x_assum(qspec_then`0` assume_tac)>>
+        rfs[EVERY_MEM,FORALL_PROD]>>
+        metis_tac[])
+      >>
+        metis_tac[])
+    >-
+      (pop_assum mp_tac>>simp[lookup_union]>>
+      reverse TOP_CASE_TAC>> strip_tac
+      >-
+        (first_x_assum drule>>rw[]>>
+        metis_tac[loc_to_pc_APPEND,code_installed_APPEND])
+      >>
+        cheat)
+    >-
+      (fs[shift_seq_def]>>pairarg_tac>>fs[]>>
+      first_x_assum(qspec_then`k'+1` assume_tac)>>rfs[]>>
+      fs[GSYM ADD1,GENLIST_CONS]>>
+      rfs[Abbr`new_code`,MAP_prog_to_section_Section_num]>>
+      fs[o_DEF])
+    >-
+      fs[shift_seq_def]
+    >>
+      (fs[shift_seq_def]>>pairarg_tac>>fs[]>>
+      first_x_assum(qspec_then`k'+1` assume_tac)>>rfs[]>>
+      fs[GSYM ADD1,GENLIST_CONS]>>
+      rfs[Abbr`new_code`,MAP_prog_to_section_Section_num]>>
+      fs[o_DEF]))>>
   conj_tac >- (
     rw[stackSemTheory.evaluate_def,flatten_def]>>
     fs[case_eq_thms]>>
@@ -1636,6 +1601,9 @@ val flatten_correct = Q.store_thm("flatten_correct",
     ntac 2 strip_tac>>simp[]>>
     fs[state_rel_def,dec_clock_def,inc_pc_def]>>
     metis_tac[])>>
+  conj_tac >- (
+    rw[stackSemTheory.evaluate_def]>>fs[state_rel_def]
+  )>>
   (* FFI *)
   conj_tac >- (
     srw_tac[][stackSemTheory.evaluate_def,flatten_def] >>
